\documentclass{article}
\usepackage{amsfonts, amsmath}

\title{Portfolio Theory Notes}
\author{Miguel Manese}
\date{}

\begin{document}
\maketitle

\begin{section}{Performance Measures}
\begin{subsection}{Returns}
\begin{description}
\item[Annual Returns] 
\item[Daily Returns] 
\item[Compounded Returns]
\end{description}
\end{subsection}

\end{section}

\begin{section}{Unsorted}
\begin{subsection}{Tangency Portfolio}
Also known as \emph{Sharpe Optimal Portfolio}. Given risk-free rate $r_f$,
risky assets $i = 1, \ldots, N$ with mean return $\mathbf{r^*}$ and return
covariance $\mathbf{V}^*$, let $\mathbf{r} = (r_f, \mathbf{r^*}')'$ and 
$\mathbf{V} = 
\begin{bmatrix}
0 & 0 \\
0 & \mathbf{V}^*
\end{bmatrix}$. Let $\mathbf{x} = (x_0, x_1, \ldots, x_N)'$ be the positions
with $\mathbf{x}'\mathbf{1} = 1$, then for some $\tau > 0$ the risk-adjusted
return for the portfolio, $R_p$, is

\begin{align}
R_p &= \mathbf{x}'\mathbf{r} - \tau \mathbf{x}'\mathbf{V}\mathbf{x} \notag\\
  & =
   x_0 r_f + \sum_{i=1}^N x_i r_i - \tau \sum_{i=1}^N \sum_{j=1}^N x_i \sigma_{i,j} x_j \notag
\end{align}

\noindent Using $x_0 = 1 - \sum_{i=1}^N x_i$ we have

\[ r_f + \sum_{i=1}^N x_i (r_i - r_f) - \tau \sum_{i=1}^N \sum_{j=1}^N x_i \sigma_{i,j} x_j \]

\noindent Maximizing

\[ \frac{\partial}{\partial x_k} R_p = 
    (r_k - r_f) + 2 \tau \sum_{j=1}^N x_k \sigma{k,j} \]

\noindent For the second term note that $k$ happens once in $i = 1, \ldots, N$
and another in $j = 1, \ldots, N$, which explains the $2$. In matrix form this
becomes

\[ \mathbf{V}^* \mathbf{x}^* = \frac{1}{2 \tau} (\mathbf{r}^* - r_f) \]

\noindent where $\mathbf{x}^* = (x_1, \dots, x_N)'$. The solution is
$\mathbf{x}^* = (\mathbf{V}^*)^{-1}$. However this is not normalized, i.e. 
$(\mathbf{x}^*)' \mathbf{1} = 1 - x_0$. To normalize

\[ \mathbf{\hat{x}}^* = \frac{1}{(\mathbf{x}^*)' \mathbf{1}} \mathbf{x}^* =
    \frac{1}{\frac{1}{2 \tau} (\mathbf{V}^*)^{-1} (\mathbf{r}^* - r_f)' \mathbf{1}}
     \frac{1}{2 \tau} (\mathbf{V}^*)^{-1} (\mathbf{r}^* - r_f) =
    \frac{1}{(\mathbf{V}^*)^{-1} (\mathbf{r}^* - r_f)' \mathbf{1}}
      (\mathbf{V}^*)^{-1} (\mathbf{r}^* - r_f) \]

\noindent i.e. $\mathbf{\hat{x}}^*$ does not depend on $\tau$.

How to show that is tangent to the efficient frontier?


\end{subsection}
\end{section}
\end{document}
